Coq/Simplicity/StaticAnalysis.v
@@ -16,9 +16,10 @@ Module StateShape.
  * doesn't crash).
  *)
 
-Definition spec {A B : Ty} (t : Term A B)  :=
-  forall x y, runMachine (@Core.eval _ _ t Naive.translate) x = Some y ->
-              stateShape x = stateShape y.
+Definition spec {A B : Ty} (t : Term A B) :=
+  forall s0 s1,
+   s0 >>- (@Core.eval _ _ t Naive.translate) ->> s1 ->
+   stateShape s0 = stateShape s1.
 
 Lemma iden_spec {A : Ty} : spec (@iden A).
 Proof.
@@ -29,102 +30,101 @@ Qed.
 Lemma comp_spec {A B C : Ty} (s : Term A B) (t : Term B C) :
  spec s -> spec t -> spec (comp s t) .
 Proof.
-intros Hs Ht x z; cbn.
-repeat rewrite runMachine_seq; cbn.
-set (x1 := Build_State _ _ _ _); specialize (Hs x1).
-destruct (runMachine _ x1) as [y0|];[cbn|discriminate].
-specialize (Hs _ (eq_refl _)).
-unfold moveFrame, runMachine at 3.
-destruct (MachineCode.MoveFrame.chk _) as [| [y1 st0]];[discriminate|cbn].
-specialize (Ht y1).
-destruct (runMachine _ y1) as [z0|];[cbn|discriminate].
-specialize (Ht _ (eq_refl _)).
-unfold dropFrame, runMachine.
-destruct (MachineCode.DropFrame.chk _) as [| [z1 st1]];[discriminate|cbn].
-intros Hz; inversion Hz as [Hz0]; rewrite <- Hz0; clear z Hz Hz0.
-destruct st0 as [l0 ctx0].
-destruct st1 as [l1 ctx1].
-destruct x as [irf arf awf iwf];
-unfold stateShape in *; cbn in *.
-inversion Hs as [[Hs0 Hs1 Hs2 Hs3 Hs4]].
-rewrite Hs0, Hs1, Hs3, Hs4.
-clear x1 Hs Hs0 Hs1 Hs2 Hs3 Hs4.
-inversion_clear Ht.
+intros Hs Ht s0 s5 Hs05.
+simpl in Hs05.
+apply seq_complete in Hs05.
+destruct Hs05 as [s4 Hs04 Hs45].
+apply seq_complete in Hs04.
+destruct Hs04 as [s3 Hs03 Hs34].
+apply seq_complete in Hs03.
+destruct Hs03 as [s2 Hs02 Hs23].
+apply seq_complete in Hs02.
+destruct Hs02 as [s1 Hs01 Hs12].
+apply newFrame_complete in Hs01.
+apply moveFrame_complete in Hs23.
+apply dropFrame_complete in Hs45.
+apply Hs in Hs12.
+apply Ht in Hs34.
+revert Hs12 Hs34.
+inversion_clear Hs01.
+inversion_clear Hs23.
+inversion_clear Hs45.
+clear.
+unfold stateShape; cbn.
+do 2 inversion 1.
 reflexivity.
 Qed.
 
 Lemma unit_spec {A : Ty} : spec (@unit A).
 Proof.
 intros x y Hxy.
-inversion_clear Hxy.
-reflexivity.
+cbn in Hxy.
+apply nop_complete in Hxy.
+congruence.
 Qed.
 
 Lemma injl_spec {A B C : Ty} (t : Term A B) :
  spec t -> spec (@injl A B C t).
 Proof.
-intros ht x y; cbn.
-repeat rewrite runMachine_seq.
-assert (Hx := stateShape_write false x).
-destruct (runMachine _ x) as [x0|];[cbn|discriminate].
-rewrite (Hx _ (refl_equal _)); clear -ht.
-assert (Hx0 := stateShape_skip (padL B C) x0).
-destruct (runMachine _ x0) as [x1|];[cbn|discriminate].
-rewrite (Hx0 _ (refl_equal _)); clear -ht.
-auto.
+intros Ht s0 s3 Hs03.
+simpl in Hs03.
+apply seq_complete in Hs03.
+destruct Hs03 as [s2 Hs02 Hs23].
+apply seq_complete in Hs02.
+destruct Hs02 as [s1 Hs01 Hs12].
+rewrite (stateShape_write _ _ _ Hs01).
+rewrite (stateShape_skip _ _ _ Hs12).
+apply (Ht _ _ Hs23).
 Qed.
 
 Lemma injr_spec {A B C : Ty} (t : Term A C) :
  spec t -> spec (@injr A B C t).
 Proof.
-intros ht x y; cbn.
-repeat rewrite runMachine_seq.
-assert (Hx := stateShape_write true x).
-destruct (runMachine _ x) as [x0|];[cbn|discriminate].
-rewrite (Hx _ (refl_equal _)); clear -ht.
-assert (Hx0 := stateShape_skip (padR B C) x0).
-destruct (runMachine _ x0) as [x1|];[cbn|discriminate].
-rewrite (Hx0 _ (refl_equal _)); clear -ht.
-auto.
+intros Ht s0 s3 Hs03.
+simpl in Hs03.
+apply seq_complete in Hs03.
+destruct Hs03 as [s2 Hs02 Hs23].
+apply seq_complete in Hs02.
+destruct Hs02 as [s1 Hs01 Hs12].
+rewrite (stateShape_write _ _ _ Hs01).
+rewrite (stateShape_skip _ _ _ Hs12).
+apply (Ht _ _ Hs23).
 Qed.
 
 Lemma bump_spec {A B : Ty} (t : Term A B) n (Ht : spec t) x y :
- runMachine (bump n (@Core.eval _ _ t Naive.translate)) x = Some y ->
+ x >>- bump n (@Core.eval _ _ t Naive.translate) ->> y ->
  stateShape x = stateShape y.
 Proof.
 unfold bump.
-repeat rewrite runMachine_seq.
-assert (Hx := stateShape_fwd n x).
-destruct (runMachine _ x) as [x0|];[cbn|discriminate].
-rewrite (Hx _ (refl_equal _)); clear -Ht.
-specialize (Ht x0).
-destruct (runMachine _ x0) as [y0|];[cbn|discriminate].
-specialize (Ht _ (refl_equal _)).
-assert (Hy := stateShape_bwd n y0).
-destruct (runMachine _ y0) as [y1|];[cbn|discriminate].
-specialize (Hy _ (refl_equal _)).
 intros Hxy.
-inversion Hxy.
-congruence.
+apply seq_complete in Hxy.
+destruct Hxy as [s2 Hxs2 Hs2y].
+apply seq_complete in Hxs2.
+destruct Hxs2 as [s1 Hxs1 Hs1s2].
+rewrite (stateShape_fwd _ _ _ Hxs1).
+rewrite (Ht _ _ Hs1s2).
+apply (stateShape_bwd _ _ _ Hs2y).
 Qed.
 
 Lemma case_spec {A B C D : Ty} (s : Term (A * C) D) (t : Term (B * C) D) :
  spec s -> spec t -> spec (case s t).
 Proof.
-intros Hs Ht x y; cbn.
-rewrite runMachine_choice.
-destruct (nextData _) as [| [[|] |] _]; try discriminate;
-apply bump_spec; auto.
+intros Hs Ht x y Hxy.
+simpl in Hxy.
+apply choice_complete in Hxy.
+destruct Hxy as [[|] _ Hxy];
+eauto using bump_spec.
 Qed.
 
 Lemma pair_spec {A B C : Ty} (s : Term A B) (t : Term A C) :
  spec s -> spec t -> spec (pair s t).
 Proof.
-intros Hs Ht x z; cbn.
-rewrite runMachine_seq.
-specialize (Hs x).
-destruct (runMachine _ x) as [y|];[|discriminate].
-rewrite (Hs y);auto.
+intros Hs Ht x z Hxz.
+simpl in Hxz.
+apply seq_complete in Hxz.
+destruct Hxz as [y Hxy Hyz].
+rewrite (Hs _ _ Hxy).
+apply (Ht _ _ Hyz).
 Qed.
 
 Lemma take_spec {A B C : Ty} (t : Term A C) :
@@ -175,90 +175,78 @@ Definition extraMemoryBound : Core.Algebra := Core.Pack (Core.Class.Class (fun A
 Definition MemoryBound {A B : Ty} (t : Term A B) x : N := stateSize x + (@Core.eval _ _ t extraMemoryBound).
 
 Definition spec {A B : Ty} (t : Term A B)  :=
-  forall x n, programMaximumMemoryResidence (@Core.eval _ _ t Naive.translate) x = Some n ->
-              n <= MemoryBound t x.
+  forall x y (tr : x >>- (@Core.eval _ _ t Naive.translate) ->> y),
+   maximumMemoryResidence (trace tr) <= MemoryBound t x.
 
 Lemma iden_spec {A : Ty} : spec (@iden A).
 Proof.
-intros x n; cbn.
-rewrite pMMR_copy.
-destruct (runMachine _ x) as [x0|];[cbn|discriminate].
-inversion_clear 1.
-unfold MemoryBound; cbn.
-rewrite N.add_0_r.
+intros x y tr.
+unfold MemoryBound.
+cbn in *.
+rewrite MMR_copy, N.add_0_r.
 reflexivity.
 Qed.
 
 Lemma comp_spec {A B C : Ty} (s : Term A B) (t : Term B C) :
  spec s -> spec t -> spec (comp s t) .
 Proof.
-intros Hs Ht x n; cbn.
-repeat rewrite pMMR_seq.
-repeat rewrite runMachine_seq.
-cbn.
-set (x0 := Build_State _ _ _ _).
-specialize (Hs x0).
-destruct (programMaximumMemoryResidence _ x0) as [nx|];[cbn|discriminate].
-specialize (Hs _ (refl_equal _)).
-assert (Hsx := StateShape.Core_spec s x0).
-destruct (runMachine _ x0) as [y|];[cbn|discriminate].
-specialize (Hsx _ (refl_equal _)).
-rewrite pMMR_moveFrame.
-unfold moveFrame, runMachine at 2 3 4.
-destruct (MachineCode.MoveFrame.chk _) as [| [y0 sty]];[discriminate|cbn].
-specialize (Ht y0).
-destruct (programMaximumMemoryResidence _ y0) as [ny|];[cbn|discriminate].
-specialize (Ht _ (refl_equal _)).
-assert (Hty := StateShape.Core_spec t y0).
-destruct (runMachine _ y0) as [z|];[cbn|discriminate].
-specialize (Hty _ (refl_equal _)).
-unfold programMaximumMemoryResidence, dropFrame.
-destruct (MachineCode.DropFrame.chk _) as [| [z0 stz]];[discriminate|cbn].
-inversion_clear 1.
-unfold MemoryBound in *; cbn.
-unfold stateSize.
-rewrite <- Hsx, <- Hty.
-fold (stateSize y0); fold (stateSize z0); fold (stateSize x0); fold (stateSize x).
+intros Hs Ht s0 s5 tr05.
+unfold MemoryBound.
+cbn in *.
+destruct (seq_complete _ _ _ _ tr05) as [s4 tr04 tr45].
+rewrite (MMR_seq _ _ _ _ _ tr04 tr45 tr05).
+destruct (seq_complete _ _ _ _ tr04) as [s3 tr03 tr34].
+rewrite (MMR_seq _ _ _ _ _ tr03 tr34 tr04).
+destruct (seq_complete _ _ _ _ tr03) as [s2 tr02 tr23].
+rewrite (MMR_seq _ _ _ _ _ tr02 tr23 tr03).
+destruct (seq_complete _ _ _ _ tr02) as [s1 tr01 tr12].
+rewrite (MMR_seq _ _ _ _ _ tr01 tr12 tr02).
 rewrite N.add_assoc.
-replace (stateSize x + _) with (stateSize x0).
- rewrite <- N.add_max_distr_l,
-         (N.max_l (stateSize y0) (stateSize z0)),
-         (N.max_r (stateSize x) (stateSize x0)),
-         (N.max_comm nx _), (N.max_assoc (stateSize x0) _ _), N.max_id,
-         N.max_assoc, N.max_comm.
-   replace (stateSize y0) with (stateSize x0) in *.
-    apply N.max_le_compat; apply N.max_lub; solve [assumption|apply N.le_add_r].
-   clear -Hsx sty.
-   unfold stateSize.
-   rewrite Hsx.
-   destruct sty as [l0 ctx0].
-   unfold stateShape, stateShapeSize; cbn.
-   rewrite fullWriteFrame_size.
-   ring.
-  unfold x0; clear.
-  destruct x as [irf arf awf iwf]; cbn.
-  unfold stateSize, stateShape, stateShapeSize; cbn.
-  repeat rewrite N.add_assoc; repeat apply N.add_le_mono_r.
-  repeat rewrite <- N.add_assoc; repeat apply N.add_le_mono_l.
-  apply N.le_add_r.
- unfold stateSize.
- rewrite Hty.
- destruct stz as [rf0 ctx0].
- destruct ctx0 as [irf arf awf iwf]; cbn.
- unfold stateShape, stateShapeSize; cbn.
- repeat rewrite N.add_assoc; repeat apply N.add_le_mono_r.
- rewrite N.add_comm.
- apply N.le_add_r.
-unfold x0; clear.
-destruct x as [irf arf awf iwf]; cbn.
-unfold stateSize, stateShape, stateShapeSize; cbn.
+rewrite MMR_newFrame, MMR_moveFrame, MMR_dropFrame.
+replace (stateSize _ + _) with (stateSize s1).
+ specialize (Hs _ _ tr12).
+ specialize (Ht _ _ tr34).
+ unfold MemoryBound, stateSize in *.
+ rewrite (StateShape.Core_spec s _ _ tr12) in *.
+ fold (stateSize s2) in *.
+ replace (stateSize s2) with (stateSize s3) in *.
+  unfold MemoryBound, stateSize in *.
+  rewrite (StateShape.Core_spec t _ _ tr34) in *.
+  rewrite N.max_comm.
+  repeat rewrite N.max_assoc.
+  rewrite N.max_id.
+  repeat rewrite <- N.max_assoc.
+  rewrite (N.max_comm _ (_ (_ tr34))).
+  repeat rewrite N.max_assoc.
+  rewrite N.max_comm.
+  repeat rewrite N.max_assoc.
+  rewrite N.max_id.
+  repeat rewrite <- N.max_assoc.
+  apply N.max_lub.
+   apply N.le_add_r.
+  rewrite <- N.add_max_distr_l.
+  apply N.max_le_compat; assumption.
+ clear - tr23.
+ apply moveFrame_complete in tr23.
+ inversion tr23.
+ unfold stateSize, stateShape, stateShapeSize.
+ cbn.
+ rewrite fullWriteFrame_size.
+ ring.
+clear - tr01.
+apply newFrame_complete in tr01.
+inversion tr01.
+unfold stateSize, stateShape, stateShapeSize.
+cbn.
 ring.
 Qed.
 
 Lemma unit_spec {A : Ty} : spec (@unit A).
 Proof.
-intros x n; unfold MemoryBound; cbn.
-inversion_clear 1.
+intros x y tr.
+unfold MemoryBound.
+cbn in *.
+destruct (trace_subproof _ _ _ _ _); cbn.
 rewrite N.add_0_r.
 reflexivity.
 Qed.
@@ -266,116 +254,81 @@ Qed.
 Lemma injl_spec {A B C : Ty} (t : Term A B) :
  spec t -> spec (@injl A B C t).
 Proof.
-intros Ht x n; cbn.
-repeat rewrite pMMR_seq.
-repeat rewrite runMachine_seq.
-rewrite pMMR_write.
-assert (Hx := stateShape_write false x).
-destruct (runMachine _ x) as [x0|];[cbn|discriminate].
-specialize (Hx _ (refl_equal _)).
-rewrite pMMR_skip.
-assert (Hx0 := stateShape_skip (padL B C) x0).
-destruct (runMachine _ x0) as [x1|];[cbn|discriminate].
-specialize (Hx0 _ (refl_equal _)).
-specialize (Ht x1).
-destruct (programMaximumMemoryResidence _ x1) as [nt|];[cbn|discriminate].
-specialize (Ht _ (refl_equal _)).
-inversion_clear 1.
-unfold MemoryBound, stateSize in *; cbn.
-rewrite Hx, Hx0; clear -Ht.
-rewrite N.max_id.
-apply N.max_lub;[assumption|].
-apply N.le_add_r.
+intros Ht s0 s3 tr03.
+unfold MemoryBound.
+cbn in *.
+destruct (seq_complete _ _ _ _ tr03) as [s2 tr02 tr23].
+rewrite (MMR_seq _ _ _ _ _ tr02 tr23 tr03).
+destruct (seq_complete _ _ _ _ tr02) as [s1 tr01 tr12].
+rewrite (MMR_seq _ _ _ _ _ tr01 tr12 tr02).
+rewrite MMR_write, MMR_skip.
+unfold stateSize.
+rewrite (stateShape_write _ _ _ tr01), N.max_id, (stateShape_skip _ _ _ tr12).
+apply N.max_lub.
+ apply N.le_add_r.
+apply Ht.
 Qed.
 
 Lemma injr_spec {A B C : Ty} (t : Term A C) :
  spec t -> spec (@injr A B C t).
 Proof.
-intros Ht x n; cbn.
-repeat rewrite pMMR_seq.
-repeat rewrite runMachine_seq.
-rewrite pMMR_write.
-assert (Hx := stateShape_write true x).
-destruct (runMachine _ x) as [x0|];[cbn|discriminate].
-specialize (Hx _ (refl_equal _)).
-rewrite pMMR_skip.
-assert (Hx0 := stateShape_skip (padR B C) x0).
-destruct (runMachine _ x0) as [x1|];[cbn|discriminate].
-specialize (Hx0 _ (refl_equal _)).
-specialize (Ht x1).
-destruct (programMaximumMemoryResidence _ x1) as [nt|];[cbn|discriminate].
-specialize (Ht _ (refl_equal _)).
-inversion_clear 1.
-unfold MemoryBound, stateSize in *; cbn.
-rewrite Hx, Hx0; clear -Ht.
-rewrite N.max_id.
-apply N.max_lub;[assumption|].
-apply N.le_add_r.
+intros Ht s0 s3 tr03.
+unfold MemoryBound.
+cbn in *.
+destruct (seq_complete _ _ _ _ tr03) as [s2 tr02 tr23].
+rewrite (MMR_seq _ _ _ _ _ tr02 tr23 tr03).
+destruct (seq_complete _ _ _ _ tr02) as [s1 tr01 tr12].
+rewrite (MMR_seq _ _ _ _ _ tr01 tr12 tr02).
+rewrite MMR_write, MMR_skip.
+unfold stateSize.
+rewrite (stateShape_write _ _ _ tr01), N.max_id, (stateShape_skip _ _ _ tr12).
+apply N.max_lub.
+ apply N.le_add_r.
+apply Ht.
 Qed.
 
-Lemma bump_spec {A B : Ty} (t : Term A B) (Ht : spec t) :
- forall x n m, programMaximumMemoryResidence (bump n (@Core.eval _ _ t Naive.translate)) x = Some m ->
-               m <= MemoryBound t x.
+Lemma bump_spec {A B : Ty} (t : Term A B) (Ht : spec t) x y n (tr : x >>- bump n (@Core.eval _ _ t Naive.translate) ->> y) :
+   maximumMemoryResidence (trace tr) <= MemoryBound t x.
 Proof.
-intros x n m.
-unfold bump.
-repeat rewrite pMMR_seq.
-repeat rewrite runMachine_seq.
-rewrite pMMR_fwd.
-assert (Hx := stateShape_fwd n x).
-destruct (runMachine _ x) as [x0|];[cbn|discriminate].
-specialize (Hx _ (refl_equal _)).
-specialize (Ht x0).
-unfold programMaximumMemoryResidence in Ht.
-unfold programMaximumMemoryResidence at 2.
-unfold runMachine.
-destruct (Core.eval _) as [[y tr0] |];[cbn in *|discriminate].
-specialize (Ht _ (refl_equal _)).
-rewrite pMMR_bwd.
-assert (Hy := stateShape_bwd n y).
-destruct (runMachine _ y) as [y0|];[cbn|discriminate].
-specialize (Hy _ (refl_equal _)).
-inversion_clear 1.
+unfold bump in tr.
+destruct (seq_complete _ _ _ _ tr) as [s2 tr02 tr23].
+rewrite (MMR_seq _ _ _ _ _ tr02 tr23).
+destruct (seq_complete _ _ _ _ tr02) as [s1 tr01 tr12].
+rewrite (MMR_seq _ _ _ _ _ tr01 tr12).
+rewrite MMR_bwd, MMR_fwd.
 unfold MemoryBound, stateSize.
-rewrite Hx.
-etransitivity;[|apply Ht].
-rewrite N.max_comm, <- N.max_assoc.
-apply N.max_lub;[reflexivity|apply MMR_bounds].
+rewrite (stateShape_fwd _ _ _ tr01).
+rewrite (N.max_comm (stateShapeSize _)), <- N.max_assoc, N.max_l.
+ apply Ht.
+apply MMR_bounds.
 Qed.
 
 Lemma case_spec {A B C D : Ty} (s : Term (A * C) D) (t : Term (B * C) D) :
  spec s -> spec t -> spec (case s t).
 Proof.
-intros Hs Ht x n; cbn.
-unfold MemoryBound; cbn.
-rewrite pMMR_choice.
+intros Hs Ht s0 s1 tr01.
+unfold MemoryBound.
+cbn in *.
 rewrite <- N.add_max_distr_l.
-destruct (nextData _) as [| [[|] |] _]; try discriminate;
- intros Hp;etransitivity;[|apply N.le_max_r| |apply N.le_max_l];
- revert Hp;apply bump_spec; assumption.
+destruct (choice_complete _ _ _ _ tr01) as [[|] Hb tr].
+ rewrite <- (trace_right _ _ _ _ tr tr01);[|assumption].
+ etransitivity;[apply bump_spec;assumption|apply N.le_max_r].
+rewrite <- (trace_left _ _ _ _ tr tr01);[|assumption].
+etransitivity;[apply bump_spec;assumption|apply N.le_max_l].
 Qed.
 
 Lemma pair_spec {A B C : Ty} (s : Term A B) (t : Term A C) :
  spec s -> spec t -> spec (pair s t).
 Proof.
-intros Hs Ht x n; unfold MemoryBound; cbn.
-rewrite pMMR_seq.
-specialize (Hs x).
-destruct (programMaximumMemoryResidence _ x) as [ns|];[cbn|discriminate].
-specialize (Hs _ (refl_equal _)).
-assert (Hsx := StateShape.Core_spec s x).
-destruct (runMachine _ x) as [y|];[cbn|discriminate].
-specialize (Hsx _ (refl_equal _)).
-specialize (Ht y).
-destruct (programMaximumMemoryResidence _ y) as [nt|];[cbn|discriminate].
-specialize (Ht _ (refl_equal _)).
-inversion_clear 1.
-rewrite N.max_comm.
-transitivity (N.max (MemoryBound s x) (MemoryBound t y)).
- apply N.max_le_compat; assumption.
-unfold MemoryBound, stateSize.
-rewrite Hsx, N.add_max_distr_l.
-reflexivity.
+intros Hs Ht s0 s2 tr02.
+unfold MemoryBound.
+cbn in *.
+destruct (seq_complete _ _ _ _ tr02) as [s1 tr01 tr12].
+rewrite (MMR_seq _ _ _ _ _ tr01 tr12 tr02).
+rewrite <- N.add_max_distr_l.
+unfold stateSize.
+rewrite (StateShape.Core_spec _ _ _ tr01) at 2.
+apply N.max_le_compat;[apply Hs|apply Ht].
 Qed.
 
 Lemma take_spec {A B C : Ty} (t : Term A C) :
@@ -408,12 +361,11 @@ Qed.
 
 Definition CellBound {A B : Ty} (t : Term A B) : N := N.of_nat (bitSize A) + N.of_nat (bitSize B) + (@Core.eval _ _ t extraMemoryBound).
 
-Lemma CellBound_correct {A B : Ty} (t : Term A B) a n:
-  programMaximumMemoryResidence (@Core.eval _ _ t Naive.translate) (fillContext emptyCtx (LocalStateBegin t a)) = Some n ->
-  n <= CellBound t.
+Lemma CellBound_correct {A B : Ty} (t : Term A B) a y
+  (tr : fillContext emptyCtx (LocalStateBegin t a) >>- @Core.eval _ _ t Naive.translate ->> y) :
+  maximumMemoryResidence (trace tr) <= CellBound t.
 Proof.
-intros Ht.
-etransitivity;[apply (Core_spec _ _ _ Ht)|].
+etransitivity;[apply (Core_spec _ _ _ tr)|].
 unfold MemoryBound, CellBound, stateSize, stateShapeSize; cbn.
 rewrite app_nil_r, encode_length, N.add_0_r, <- plus_n_O.
 reflexivity.
